theories/WPLifted.v
@@ -49,10 +49,15 @@ Delimit Scope wp_scope with wp.
 Definition Weakestpre (T:forall `{Enc A},hprop->(A->hprop)->Prop) : Formula :=
   fun A (EA:Enc A) => weakestpre T.
 
-(** Lifted version of [wp_triple] *)
+(** Lifted version of [wp] *)
 
-Definition Wp_Triple (t:trm) : Formula :=
+Definition Wp (t:trm) : Formula :=
   Weakestpre (@Triple t).
+
+(** Lifted version of [wpsubst E t] *)
+
+Definition Wpsubst (E:ctx) (t:trm) : Formula :=
+  Wp (isubst E t).
 
 
 (* ---------------------------------------------------------------------- *)
@@ -62,14 +67,15 @@ Definition Wp_Triple (t:trm) : Formula :=
 
 Definition Formula_typed `{Enc A1} (F:(A1->hprop)->hprop) : Formula :=
   fun A2 (EA2:Enc A2) (Q:A2->hprop) =>
-    \exists (Q':A1->hprop), F Q' \* \[PostChange Q' Q].
+    \exists (Q':A1->hprop), F Q' \* \[RetypePost Q' Q].
 
-(** [Wp_cast X Q] applies a postcondition [Q] of type [A2->hprop] to a value
+(** [Wpgen_cast X Q] applies a postcondition [Q] of type [A2->hprop] to a value
     [X] of type [A1], with [X] converted on-the-fly to a value of type [A2]. *)
 
-Definition Wp_cast `{Enc A1} (X:A1) A2 (EA2:Enc A2) (Q:A2->hprop) : hprop :=
+Definition Wpgen_cast `{Enc A1} (X:A1) A2 (EA2:Enc A2) (Q:A2->hprop) : hprop :=
   \exists (Y:A2), \[enc X = enc Y] \* Q Y.
 
+(* TODO: is Wpgen_cast not similar to (Wpgen_val `X) *)
 
 (* ---------------------------------------------------------------------- *)
 (* ** Definition of [Local] for WP *)
@@ -96,10 +102,10 @@ Hint Resolve flocal_Local.
 (* ---------------------------------------------------------------------- *)
 (* ** Tag for improved pretty-printing of CF *)
 
-Definition is_Wp (F:Formula) : Formula := F.
+Definition Wptag (F:Formula) : Formula := F.
 
 Notation "'`' F" :=
-  ((is_Wp F%wp))
+  ((Wptag F%wp))
   (at level 69, F at level 100, format "'`' F") : wp_scope.
 
 
@@ -109,346 +115,214 @@ Notation "'`' F" :=
 (** These auxiliary definitions give the characteristic formula
     associated with each term construct. *)
 
-Definition Wp_fail : Formula :=
+Definition Wpgen_fail : Formula :=
   Local (fun A (EA:Enc A) Q =>
     \[False]).
 
-Definition Wp_val (v:val) : Formula :=
+Definition Wpgen_val (v:val) : Formula :=
   Local (fun A (EA:Enc A) Q =>
     \exists (V:A), \[v = enc V] \* Q V).
 
 (* DEPRECATED
-Definition Wp_val_typed `{EA1:Enc A1} (V:A1) : Formula :=
+Definition Wpgen_val_typed `{EA1:Enc A1} (V:A1) : Formula :=
   Local (fun A (EA:Enc A) Q => Q V1).
 *)
 
-Definition WP_var (E:ctx) (x:var) : Formula :=
+Definition Wpaux_var (E:ctx) (x:var) : Formula :=
   match Ctx.lookup x E with
-  | None => `Wp_fail
-  | Some v => `Wp_val v
+  | None => `Wpgen_fail
+  | Some v => `Wpgen_val v
   end.
 
-(** DEPRECATED
-    [Wp_var] prevents [simpl] from simplifying context lookups, hence we
-    inline its definition at the place of use, using a notation. 
-
-Notation "'Wp_var'' E x" :=
-  (match Ctx.lookup x E with
-  | None => Wp_fail
-  | Some v => Wp_val v
-  end) (at level 37, E at level 0, x at level 0).
-*)
-
-Definition Wp_let (F1:Formula) (F2of:forall `{EA1:Enc A1},A1->Formula) : Formula :=
+Definition Wpgen_let (F1:Formula) (F2of:forall `{EA1:Enc A1},A1->Formula) : Formula :=
   Local (fun A (EA:Enc A) Q =>
     \exists (A1:Type) (EA1:Enc A1),
       ^F1 (fun (X:A1) => ^(F2of X) Q)).
 
-Definition Wp_let_typed `{EA1:Enc A1} (F1:Formula) (F2of:A1->Formula) : Formula :=
+Definition Wpgen_let_typed `{EA1:Enc A1} (F1:Formula) (F2of:A1->Formula) : Formula :=
   Local (fun `{Enc A} Q =>
     ^F1 (fun (X:A1) => ^(F2of X) Q)).
 
-Definition Wp_seq (F1 F2:Formula) : Formula :=
+Definition Wpgen_seq (F1 F2:Formula) : Formula :=
   Local (fun A (EA:Enc A) Q =>
     ^F1 (fun (X:unit) => ^F2 Q)).
 
-Definition Wp_letval (v:val) (F2of:forall `{EA1:Enc A1},A1->Formula) : Formula :=
+Definition Wpgen_letval (v:val) (F2of:forall `{EA1:Enc A1},A1->Formula) : Formula :=
   Local (fun A (EA:Enc A) Q =>
     \exists (A1:Type) (EA1:Enc A1) (V:A1), \[v = enc V] \* ^(F2of V) Q).
 
-Definition Wp_letval_typed `{EA1:Enc A1} (v:val) (F2of:A1->Formula) : Formula :=
+Definition Wpgen_letval_typed `{EA1:Enc A1} (v:val) (F2of:A1->Formula) : Formula :=
   Local (fun A (EA:Enc A) Q =>
     \exists (V:A1), \[v = enc V] \* ^(F2of V) Q).
 
-(* DEPRECATED
-Definition Wp_getval' Wp (E:ctx) (t1:trm) (F2of:forall A1 {EA1:Enc A1},A1->Formula) : Formula :=
+Definition Wpaux_getval_typed Wpgen (E:ctx) `{EA1:Enc A1} (t1:trm) (F2of:A1->Formula) : Formula :=
   match t1 with
-  | trm_val v => Wp_letval v F2of
+  | trm_val v => `Wpgen_letval_typed v F2of
   | trm_var x => match Ctx.lookup x E with
-                        | Some v => Wp_letval v F2of
-                        | None => Wp_fail
+                        | Some v => `Wpgen_letval_typed v F2of
+                        | None => `Wpgen_fail
                         end
-  | _ => Wp_let (Wp E t1) F2of
-  end.
-*)
-
-Definition WP_getval_typed Wp (E:ctx) `{EA1:Enc A1} (t1:trm) (F2of:A1->Formula) : Formula :=
-  match t1 with
-  | trm_val v => `Wp_letval_typed v F2of
-  | trm_var x => match Ctx.lookup x E with
-                        | Some v => `Wp_letval_typed v F2of
-                        | None => `Wp_fail
-                        end
-  | _ => `Wp_let_typed (Wp E t1) F2of
+  | _ => `Wpgen_let_typed (Wpgen E t1) F2of
   end.
 
-(* NEEDED?
-Definition Wp_getval_val Wp (E:ctx) (t1:trm) (F2of:val->Formula) : Formula :=
+Definition Wpaux_getval Wpgen (E:ctx) (t1:trm) (F2of:val->Formula) : Formula :=
   match t1 with
   | trm_val v => F2of v
   | trm_var x => match Ctx.lookup x E with
                         | Some v => F2of v
-                        | None => Wp_fail
+                        | None => `Wpgen_fail
                         end
-  | _ => Wp_let_typed (Wp E t1) F2of
-  end.
-*)
-Definition WP_getval Wp (E:ctx) (t1:trm) (F2of:val->Formula) : Formula :=
-  match t1 with
-  | trm_val v => F2of v
-  | trm_var x => match Ctx.lookup x E with
-                        | Some v => F2of v
-                        | None => `Wp_fail
-                        end
-  | _ => `Wp_let (Wp E t1) (fun `{EA1:Enc A1} (V1:A1) => F2of (``V1))
+  | _ => `Wpgen_let (Wpgen E t1) (fun `{EA1:Enc A1} (V1:A1) => F2of (``V1))
   end.
 
-Definition WP_getval_val := WP_getval.
+Definition Wpaux_getval_val := Wpaux_getval.
 
-Definition WP_getval_int Wp (E:ctx) (t1:trm) (F2of:int->Formula) : Formula :=
+Definition Wpaux_getval_int Wpgen (E:ctx) (t1:trm) (F2of:int->Formula) : Formula :=
   match t1 with
   | trm_val (val_int n) => F2of n
-  | _ => WP_getval_typed Wp E t1 F2of
+  | _ => Wpaux_getval_typed Wpgen E t1 F2of
   end.
 
-Definition WP_constr Wp (E:ctx) (id:idconstr) : list val -> list trm -> Formula := 
+Definition Wpaux_constr Wpgen (E:ctx) (id:idconstr) : list val -> list trm -> Formula := 
   fix mk (rvs : list val) (ts : list trm) : Formula :=
     match ts with
-    | nil => `Wp_val (val_constr id (List.rev rvs))
-    | t1::ts' => WP_getval Wp E t1 (fun v1 => mk (v1::rvs) ts')
-    (* DEPRECATED Wp_getval_val wp E t1 (fun v1 => mk (v1::rvs) ts') *)
+    | nil => `Wpgen_val (val_constr id (List.rev rvs))
+    | t1::ts' => Wpaux_getval Wpgen E t1 (fun v1 => mk (v1::rvs) ts')
+    (* DEPRECATED Wpgen_getval_val wp E t1 (fun v1 => mk (v1::rvs) ts') *)
     end.
 
-(* DEPRECATED
-Definition Wp_unop_int (v1:val) (F:int->int) : Formula := 
-  Local (Formula_typed (fun (Q:int->hprop) =>
-    \exists n1, \[v1 = val_int n1] \* Q (F n1))).
+Definition Wpgen_app (t:trm) : Formula := 
+  Local (Wp t).
 
-Definition Wp_unop_bool (v1:val) (F:bool->bool) : Formula := 
-  Local (Formula_typed (fun (Q:bool->hprop) =>
-    \exists b1, \[v1 = val_bool b1] \* Q (F b1))).
-
-Definition Wp_binop_int (v1 v2:val) (F:int->int->int) : Formula :=
-  Local (Formula_typed (fun (Q:int->hprop) =>
-    \exists n1 n2, \[v1 = val_int n1 /\ v2 = val_int n2] \* Q (F n1 n2))).
-*)
-
-Definition Wp_app (t:trm) : Formula := 
-  Local (Wp_Triple t).
-
-(* TODO
-  | val_prim val_opp, (v1::nil) => Wp_unop_int v1 (fun n1 => - n1)
-  | val_prim val_neg, (v1::nil) => Wp_unop_bool v1 (fun b1 => neg b1)
-  | val_prim val_eq, (v1::v2::nil) => Wp_val (isTrue (v1 = v2))
-  | val_prim val_neq, (v1::v2::nil) => Wp_val (isTrue (v1 <> v2))
-  | val_prim val_add, (v1::v2::nil) => Wp_binop_int v1 v2 (fun n1 n2 => n1 + n2)
-  | val_prim val_sub, (v1::v2::nil) => Wp_binop_int v1 v2 (fun n1 n2 => n1 - n2)
-  | val_prim val_mul, (v1::v2::nil) => Wp_binop_int v1 v2 (fun n1 n2 => n1 * n2)
-*)
-(* not included: arithmetic comparisons *)
-
-Definition WP_apps Wp (E:ctx) (v0:func) : list val -> list trm -> Formula := 
+Definition Wpaux_apps Wpgen (E:ctx) (v0:func) : list val -> list trm -> Formula := 
   (fix mk (rvs : list val) (ts : list trm) : Formula :=
     match ts with
-    | nil => `Wp_app (trm_apps v0 (trms_vals (List.rev rvs)))
-    | t1::ts' => WP_getval Wp E t1 (fun v1 => mk (v1::rvs) ts')
+    | nil => `Wpgen_app (trm_apps v0 (trms_vals (List.rev rvs)))
+    | t1::ts' => Wpaux_getval Wpgen E t1 (fun v1 => mk (v1::rvs) ts')
     end).
 
-Definition WP_apps_or_prim Wp (E:ctx) (t0:trm) (ts:list trm) : Formula :=
+Definition Wpaux_apps_or_prim Wpgen (E:ctx) (t0:trm) (ts:list trm) : Formula :=
   match t0, ts with
   | trm_val (val_prim val_add), (t1::t2::nil) => 
-     WP_getval_int Wp E t1 (fun n1 => 
-       WP_getval_int Wp E t2 (fun n2 => 
+     Wpaux_getval_int Wpgen E t1 (fun n1 => 
+       Wpaux_getval_int Wpgen E t2 (fun n2 => 
          `Formula_typed (fun (Q:int->hprop) => Q (n1 + n2))))
-  | _,_ => WP_getval_val Wp E t0 (fun v0 => WP_apps Wp E v0 nil ts)
+  | _,_ => Wpaux_getval_val Wpgen E t0 (fun v0 => Wpaux_apps Wpgen E v0 nil ts)
   end.
 
-Definition Wp_if_val (b:bool) (F1 F2:Formula) : Formula :=
+Definition Wpgen_if_val (b:bool) (F1 F2:Formula) : Formula :=
   Local (fun `{Enc A} Q =>
     if b then ^F1 Q else ^F2 Q).
 
-Definition WP_if (F0 F1 F2:Formula) : Formula :=
-  `Wp_let_typed F0 (fun (b:bool) => `Wp_if_val b F1 F2).
+Definition Wpaux_if (F0 F1 F2:Formula) : Formula :=
+  `Wpgen_let_typed F0 (fun (b:bool) => `Wpgen_if_val b F1 F2).
 
-Definition Wp_while (F1 F2:Formula) : Formula :=
+Definition Wpgen_while (F1 F2:Formula) : Formula :=
   Local (`Formula_typed (fun (Q:unit->hprop) =>
     \forall (R:Formula),
-    let F := WP_if F1 (Wp_seq F2 R) (Wp_val val_unit) in
+    let F := Wpaux_if F1 (Wpgen_seq F2 R) (Wpgen_val val_unit) in
     \[ flocal (@R unit _) /\ (forall Q', ^F Q' ==> ^R Q')] \-* (^R Q))).
+    (* TODO: use a lifted version of flocal *)
 
-Definition Wp_for_int (n1 n2:int) (F1:int->Formula) : Formula := 
+Definition Wpgen_for_int (n1 n2:int) (F1:int->Formula) : Formula := 
   Local (Formula_typed (fun (Q:unit->hprop) =>
     \forall (S:int->Formula),
-    let F i := If (i <= n2) then (`Wp_seq (F1 i) (S (i+1)))
-                            else (`Wp_val val_unit) in
-    \[ (forall i, flocal (S i unit _)) /\ (forall i Q', ^(F i) Q' ==> ^(S i) Q')] \-* (^(S n1) Q))).
+    let F i := If (i <= n2) then (`Wpgen_seq (F1 i) (S (i+1)))
+                            else (`Wpgen_val val_unit) in
+    \[   (forall i, flocal (S i unit _)) 
+      /\ (forall i Q', ^(F i) Q' ==> ^(S i) Q')] \-* (^(S n1) Q))).
+     (* TODO: use a lifted version of flocal_pred *)
 
-Definition Wp_case_val (F1:Formula) (P:Prop) (F2:Formula) : Formula :=
+Definition Wpgen_case_val (F1:Formula) (P:Prop) (F2:Formula) : Formula :=
   Local (fun `{Enc A} Q =>
     hand (^F1 Q) (\[P] \-* ^F2 Q)).
 
-Definition WP_match Wp (E:ctx) (v:val) : list (pat*trm) ->  Formula :=
+Definition Wpaux_match Wpgen (E:ctx) (v:val) : list (pat*trm) ->  Formula :=
   fix mk (pts:list(pat*trm)) : Formula :=
     match pts with
-    | nil => `Wp_fail
+    | nil => `Wpgen_fail
     | (p,t)::pts' =>
         let xs := patvars p in
         let F1 A (EA:Enc A) (Q:A->hprop) := 
            hforall_vars (fun G => let E' := (Ctx.app G E) in
-              \[v = patsubst G p] \-* ^(Wp E' t) Q) Ctx.empty xs in
+              \[v = patsubst G p] \-* ^(Wpgen E' t) Q) Ctx.empty xs in
         let P := forall_vars (fun G => v <> patsubst G p) Ctx.empty xs in
-        Wp_case_val F1 P (mk pts')
+        Wpgen_case_val F1 P (mk pts')
     end.
-  (* Warning: the body of the cons case above, if put in an auxiliary definition,
-     no longer simplifies well using [xwp_simpl] *)
+  (* Note: the body of the cons case above, if put in an auxiliary definition,
+     does not appear to simplify well using [xwp_simpl] *)
 
-
-(*
-Definition fand (F1 F2:Formula) : Formula :=
-  Local (fun `{Enc A} Q => hand (^F1 Q) (^F2 Q)).
-
-
-Definition Wp_case_val Wp (E:ctx) (v1:val) (p:pat) (t2:trm) (F3:Formula) : Formula :=
-  let F1 A (EA:Enc A) (Q:A->hprop) := 
-     hprop_forall_pat_vars (fun G => \[v1 = patsubst G p] \-* ^(Wp (Ctx.app G E) t2) Q) Ctx.empty (patvars p) in
-  let F2 A (EA:Enc A) (Q:A->hprop) := 
-     let P := prop_forall_pat_vars (fun G => v1 <> patsubst G p) Ctx.empty (patvars p) in
-     (\[P] \-* ^F3 Q) in
-  fand F1 F2.
-*)
-
-(* not unfolding all
-
-Definition Wp_case_val Wp (E:ctx) (v1:val) (p:pat) (t2:trm) (F3:Formula) : Formula :=
-  let F1 A (EA:Enc A) (Q:A->hprop) := 
-     hprop_forall_pat_vars (fun G => \[v1 = patsubst G p] \-* ^(Wp (Ctx.app G E) t2) Q) Ctx.empty (patvars p) in
-  let P2 := prop_forall_pat_vars (fun G => v1 <> patsubst G p) Ctx.empty (patvars p) in
-  Local (fun `{Enc A} Q => hand (^F1 Q) (\[P2] \-* ^F3 Q) ).
-
-
-Definition Wp_case_val Wp (E:ctx) (v1:val) (p:pat) (t2:trm) (t3:trm) : Formula :=
-  Local (fun `{Enc A} Q => 
-    hand (hprop_forall_pat_vars Ctx.empty (patvars p) (fun G => \[v1 = patsubst G p] \-* ^(Wp (Ctx.app G E) t2) Q))
-         (\[prop_forall_pat_vars Ctx.empty (patvars p) (fun G => v1 <> patsubst G p)] \-* ^(Wp E t3) Q) ).
-*)
-
-(* Not computing so well
-Fixpoint hprop_forall_pat_vars (G:ctx) (xs:vars) (Hof:ctx->hprop) : hprop :=
-  match xs with
-  | nil => Hof G
-  | x::xs' => \forall (X:val), hprop_forall_pat_vars (Ctx.add x X G) xs' Hof
-  end.
-
-*)
-
-
-(* Factorized yet obfuscated version:
-
-Definition forall_pat_vars (T:Type) (Forall:(val->T)->T) (K:ctx->T) : ctx -> vars -> T :=
-  fix mk (G:ctx) (xs:vars) : T :=
-    match xs with
-    | nil => K G
-    | x::xs' => Forall (fun (X:val) => mk (Ctx.add x X G) xs')
-    end.
-
-Definition pforall (F:val->Prop) : Prop := 
-  forall (v:val), F v.
-
-Definition Wp_case_val (v1:val) (p:pat) (F1of:ctx->Formula) (F2:Formula) : Formula :=
-  Local (fun `{Enc A} Q => 
-    hand (forall_pat_vars (@hforall val) (fun G => \[v1 = patsubst G p] \-* ^(F1of G) Q) Ctx.empty (patvars p) )
-         (\[forall_pat_vars pforall (fun G => v1 <> patsubst G p) Ctx.empty (patvars p)] \-* ^F2 Q) ).
-
-*)
-
-
-
-(* DEPRECATED
-Definition Wp_case_val `{EA1:Enc A1} (V1:A1) (p:pat) (F1of:ctx->Formula) (F2:Formula) : Formula :=
-  Local (fun `{Enc A} Q => 
-    hand (\forall (G:ctx), \[Ctx.dom G = patvars p /\ (enc V1) = patsubst G p] \-* ^(F1of G) Q)
-         (\[forall (G:ctx), Ctx.dom G = patvars p -> (enc V1) <> patsubst G p] \-* ^F2 Q) ).
-
-
-Definition Wp_case_val (v1:val) (p:pat) (F1of:ctx->Formula) (F2:Formula) : Formula :=
-  Local (fun `{Enc A} Q => 
-    hand (\forall (G:ctx), \[Ctx.dom G = patvars p /\ v1 = patsubst G p] \-* ^(F1of G) Q)
-         (\[forall (G:ctx), Ctx.dom G = patvars p -> v1 <> patsubst G p] \-* ^F2 Q) ).
-*)
 
 (* ---------------------------------------------------------------------- *)
 (* ** Definition of the CF generator *)
 
-Fixpoint Wp (E:ctx) (t:trm) : Formula :=
-  let aux := Wp E in
+Fixpoint Wpgen (E:ctx) (t:trm) : Formula :=
+  let aux := Wpgen E in
   match t with
-  | trm_val v => `Wp_val v
-  | trm_var x => WP_var E x
+  | trm_val v => `Wpgen_val v
+  | trm_var x => Wpaux_var E x
   | trm_fixs f xs t1 =>
       match xs with 
-      | nil => `Wp_fail
-      | _ => `Wp_val (val_fixs f xs (isubst (Ctx.rem_vars xs (Ctx.rem f E)) t1))
+      | nil => `Wpgen_fail
+      | _ => `Wpgen_val (val_fixs f xs (isubst (Ctx.rem_vars xs (Ctx.rem f E)) t1))
       end
-  | trm_constr id ts => WP_constr Wp E id nil ts
+  | trm_constr id ts => Wpaux_constr Wpgen E id nil ts
   | trm_if t0 t1 t2 =>
-     WP_getval_typed Wp E t0 (fun b0 => 
-       `Wp_if_val b0 (aux t1) (aux t2))
+     Wpaux_getval_typed Wpgen E t0 (fun b0 => 
+       `Wpgen_if_val b0 (aux t1) (aux t2))
   | trm_let z t1 t2 =>
      match z with
-     | bind_anon => `Wp_seq (aux t1) (aux t2)
-     | bind_var x => `Wp_let (aux t1) (fun `{EA:Enc A} (X:A) => Wp (Ctx.add x (enc X) E) t2)
+     | bind_anon => `Wpgen_seq (aux t1) (aux t2)
+     | bind_var x => `Wpgen_let (aux t1) (fun `{EA:Enc A} (X:A) => Wpgen (Ctx.add x (enc X) E) t2)
      end
-  | trm_apps t0 ts => WP_getval_val Wp E t0 (fun v0 => WP_apps Wp E v0 nil ts)
-      (* Wp_apps_or_prim Wp E t0 ts *)
-  | trm_while t1 t2 => `Wp_while (aux t1) (aux t2)
+  | trm_apps t0 ts => Wpaux_getval_val Wpgen E t0 (fun v0 => Wpaux_apps Wpgen E v0 nil ts)
+      (* Wpgen_apps_or_prim Wpgen E t0 ts *)
+  | trm_while t1 t2 => `Wpgen_while (aux t1) (aux t2)
   | trm_for x t1 t2 t3 => 
-     WP_getval_typed Wp E t1 (fun n1 =>
-       WP_getval_typed Wp E t2 (fun n2 =>
-         `Wp_for_int n1 n2 (fun n => Wp (Ctx.add x (enc n) E) t3)))
+     Wpaux_getval_typed Wpgen E t1 (fun n1 =>
+       Wpaux_getval_typed Wpgen E t2 (fun n2 =>
+         `Wpgen_for_int n1 n2 (fun n => Wpgen (Ctx.add x (enc n) E) t3)))
   | trm_match t0 pts =>
-      WP_getval Wp E t0 (fun v0 =>
-        WP_match Wp E v0 pts)
-  | trm_fail => `Wp_fail
+      Wpaux_getval Wpgen E t0 (fun v0 =>
+        Wpaux_match Wpgen E v0 pts)
+  | trm_fail => `Wpgen_fail
   end.
-
-(* LATER: uniformiser t0 vs t1 for trm_if *)
 
 
 (* ********************************************************************** *)
 (* * Soundness proof *)
 
-
 (* ---------------------------------------------------------------------- *)
 (* ** Properties of semantical wp *)
 
-(** [Wp_Triple t] is a local formula *)
+(** [Wp t] is a local formula *)
 
-Lemma flocal_Wp_Triple : forall `{EA:Enc A} t,
-  flocal ((Wp_Triple t) A EA).
+Lemma flocal_Wp : forall `{EA:Enc A} t,
+  flocal ((Wp t) A EA).
 Proof using.
-  intros. unfolds Wp_Triple. unfolds Weakestpre.
+  intros. unfolds Wp. unfolds Weakestpre.
   applys flocal_weakestpre. applys is_local_Triple.
 Qed.
 
 (** Equivalence between a [triple] and its weakest-precondition presentation. *)
 
-Lemma Triple_eq_himpl_Wp_Triple : forall `{EA:Enc A} H (Q:A->hprop) t,
-  Triple t H Q = (H ==> ^(Wp_Triple t) Q).
+Lemma Triple_eq_himpl_Wp : forall `{EA:Enc A} H (Q:A->hprop) t,
+  Triple t H Q = (H ==> ^(Wp t) Q).
 Proof using. intros. applys weakestpre_eq. applys is_local_Triple. Qed.
 
 (** Reformulation of the left-to-right implication above in the form
     of an entailment. *)
 
-Lemma qimpl_Wp_Triple : forall t `{EA:Enc A} F,
+Lemma qimpl_Wp : forall t `{EA:Enc A} F,
   (forall Q, Triple t (F Q) Q) ->
-  F ===> ((Wp_Triple t) A EA).
-Proof using. introv M. intros Q. rewrite~ <- Triple_eq_himpl_Wp_Triple. Qed.
+  F ===> ((Wp t) A EA).
+Proof using. introv M. intros Q. rewrite~ <- Triple_eq_himpl_Wp. Qed.
 
 (** Another formulation of the same corrolary --- not currently used *)
-Lemma himpl_Wp_Triple_of_Triple : forall A `{EA:Enc A} (Q1:A->hprop) t H1,
+Lemma himpl_Wp_of_Triple : forall A `{EA:Enc A} (Q1:A->hprop) t H1,
   Triple t H1 Q1 ->
-  H1 ==> ^(Wp_Triple t) Q1.
-Proof using. introv M. rewrite* <- Triple_eq_himpl_Wp_Triple. Qed.
+  H1 ==> ^(Wp t) Q1.
+Proof using. introv M. rewrite* <- Triple_eq_himpl_Wp. Qed.
 
 
 (* ---------------------------------------------------------------------- *)
@@ -477,7 +351,7 @@ Proof using.
 Qed.
 
 (** The tactic [remove_Local] applies to goal of the form [triple t (local F Q) Q]
-    and turns it into [triple t (F Q) Q] for a fresh [Q],  then calls [xpull] *)
+    and turns it into [triple t (F Q) Q] for a fresh [Q]. *)
 
 Ltac remove_Local :=
   match goal with |- @Triple _ _ _ _ ?Q =>
@@ -487,215 +361,220 @@ Ltac remove_Local :=
 (* ---------------------------------------------------------------------- *)
 (* ** Soundness of [wp] *)
 
-(** [Wp_Triple_ E t] is a shorthand for [wp_triple (isubst E t)] *)
-
-Definition Wp_Triple_ E t :=
-  Wp_Triple (isubst E t).
-
-(** [Wp_sound t] asserts that [wp] is sound for all contexts [E],
-    in the sense that the syntactic wp entails the semantics wp. *)
-(*
-Definition Wp_sound t := forall E `{EA:Enc A} (Q:A->hprop),
-  ^(Wp E t) Q ==> ^(Wp_Triple_ E t) Q.
-*)
+(* [F1 ====> F2] asserts that a Formula entails another one at all types. *)
 
 Notation "F1 ====> F2" := (forall `{EA:Enc A}, F1 A EA ===> F2 A EA)
   (at level 67).
 
-(*
-Definition Wp_sound t := forall E `{EA:Enc A},
-  (Wp E t) A EA ===> (Wp_Triple_ E t) A EA.
-*)
-Definition Wp_sound t := forall E,
-  (Wp E t) ====> (Wp_Triple_ E t).
 
+(** [Wpgen_sound t] asserts that [wp] is sound for all contexts [E],
+    in the sense that the syntactic wp entails the semantics wp.
+    The definition below is equivalent to:
+[[
+    Definition Wpgen_sound t := 
+       forall E `{EA:Enc A} (Q:A->hprop),
+       ^(Wpgen E t) Q ==> ^(Wpsubst E t) Q.
+]]
+*)
+
+Definition Wpgen_sound t := forall E,
+  (Wpgen E t) ====> (Wpsubst E t).
+
+(** Lemma for [wpgen_fail] *)
+
+Lemma himpl_Wpgen_fail_l : forall `{EA:Enc A} (Q:A->hprop) H,
+  ^Wpgen_fail Q ==> H.
+Proof using. intros. unfold Wpgen_fail, Local, local. hpull. Qed.
+
+(* TODO: use lemma below for all occurences of wpgen_fail *)
+Lemma Triple_Wpgen_fail : forall t Q Q',
+  Triple t (^Wpgen_fail Q) Q'.
+Proof using. 
+  intros. apply triple_of_wp. applys himpl_wpgen_fail_l.
+Qed.
 
 (** Soundness of the [wp] for the various constructs *)
 
-Lemma Wp_sound_var : forall x,
-  Wp_sound (trm_var x).
+Lemma Wpgen_sound_var : forall x,
+  Wpgen_sound (trm_var x).
 Proof using.
-  intros. intros E A EA. simpl. applys qimpl_Wp_Triple.
-  intros Q. unfold Wp_var. simpl. destruct (Ctx.lookup x E).
+  intros. intros E A EA. simpl. applys qimpl_Wp.
+  intros Q. unfold Wpgen_var. simpl. destruct (Ctx.lookup x E).
   { remove_Local. xpull ;=> V EQ. applys* Triple_val. }
   { remove_Local. xpull*. intros; false. 
     (* TODO: decide whether xpull should automatically discard goal
        when extracting false *) }
 Qed.
 
-Lemma Wp_sound_val : forall v,
-  Wp_sound (trm_val v).
+Lemma Wpgen_sound_val : forall v,
+  Wpgen_sound (trm_val v).
 Proof using.
-  intros. intros E A EA. simpl. applys qimpl_Wp_Triple.
+  intros. intros E A EA. simpl. applys qimpl_Wp.
   intros Q. remove_Local. xpull ;=> V EQ.
   simpl. intros. applys* Triple_val.
 Qed.
 
-Lemma Wp_sound_fix : forall f x t,
-  Wp_sound (trm_fix f x t).
+Lemma Wpgen_sound_fix : forall f x t,
+  Wpgen_sound (trm_fix f x t).
 Proof using.
-  intros. intros E A EA. simpl. applys qimpl_Wp_Triple.
+  intros. intros E A EA. simpl. applys qimpl_Wp.
   intros Q. remove_Local. xpull ;=> V EQ. simpl.
   applys Triple_enc_val_inv (fun r => \[r = enc V] \* (Q V)).
   { applys Triple_fix. rewrite EQ. hsimpl~. }
   { hpull ;=> X EX. subst X. hsimpl~. }
 Qed.
 
-Lemma Wp_sound_if : forall F1 F2 F3 E t1 t2 t3,
-  F1 ====> (Wp_Triple_ E t1) ->
-  F2 ====> (Wp_Triple_ E t2) ->
-  F3 ====> (Wp_Triple_ E t3) ->
-  Wp_if F1 F2 F3 ====> Wp_Triple_ E (trm_if t1 t2 t3).
+Lemma Wpgen_sound_if : forall F0 F1 F2 E t0 t1 t2,
+  F0 ====> (Wpsubst E t0) ->
+  F1 ====> (Wpsubst E t1) ->
+  F2 ====> (Wpsubst E t2) ->
+  Wpgen_if F0 F1 F2 ====> Wpsubst E (trm_if t0 t1 t2).
 Proof using.
-  introv M1 M2 M3. intros A EA. applys qimpl_Wp_Triple. intros Q.
+  introv M0 M1 M2. intros A EA. applys qimpl_Wp. intros Q.
   remove_Local. xpull. intros _. simpl. applys Triple_if.
-  { rewrite Triple_eq_himpl_Wp_Triple. applys* M1. }
+  { rewrite Triple_eq_himpl_Wp. applys* M0. }
   { intros b. simpl. remove_Local. case_if.
-    { rewrite Triple_eq_himpl_Wp_Triple. applys* M2. }
-    { rewrite Triple_eq_himpl_Wp_Triple. applys* M3. } }
+    { rewrite Triple_eq_himpl_Wp. applys* M1. }
+    { rewrite Triple_eq_himpl_Wp. applys* M2. } }
 Qed.
 
-Lemma Wp_sound_seq : forall F1 F2 E t1 t2,
-  F1 ====> Wp_Triple_ E t1 ->
-  F2 ====> Wp_Triple_ E t2 ->
-  Wp_seq F1 F2 ====> Wp_Triple_ E (trm_seq t1 t2).
+Lemma Wpgen_sound_seq : forall F1 F2 E t1 t2,
+  F1 ====> Wpsubst E t1 ->
+  F2 ====> Wpsubst E t2 ->
+  Wpgen_seq F1 F2 ====> Wpsubst E (trm_seq t1 t2).
 Proof using.
-  introv M1 M2. intros A EA. applys qimpl_Wp_Triple. intros Q.
+  introv M1 M2. intros A EA. applys qimpl_Wp. intros Q.
   remove_Local. simpl. applys Triple_seq.
-  { rewrite Triple_eq_himpl_Wp_Triple. applys* M1. }
-  { rewrite Triple_eq_himpl_Wp_Triple. applys* M2. }
+  { rewrite Triple_eq_himpl_Wp. applys* M1. }
+  { rewrite Triple_eq_himpl_Wp. applys* M2. }
 Qed.
 
-Lemma Wp_sound_let : forall (F1:Formula) (F2of:forall `{EA1:Enc A1},A1->Formula) E (x:var) t1 t2,
-  F1 ====> Wp_Triple_ E t1 ->
-  (forall `{EA:Enc A} (X:A), F2of X ====> Wp_Triple_ (Ctx.add x (enc X) E) t2) ->
-  Wp_let F1 (@F2of) ====> Wp_Triple_ E (trm_let x t1 t2).
+Lemma Wpgen_sound_let : forall (F1:Formula) (F2of:forall `{EA1:Enc A1},A1->Formula) E (x:var) t1 t2,
+  F1 ====> Wpsubst E t1 ->
+  (forall `{EA:Enc A} (X:A), F2of X ====> Wpsubst (Ctx.add x (enc X) E) t2) ->
+  Wpgen_let F1 (@F2of) ====> Wpsubst E (trm_let x t1 t2).
 Proof using.
   Opaque Ctx.rem.
-  introv M1 M2. intros A EA. applys qimpl_Wp_Triple. intros Q.
+  introv M1 M2. intros A EA. applys qimpl_Wp. intros Q.
   remove_Local. xpull ;=> A1 EA1. simpl. applys Triple_let.
-  { rewrite Triple_eq_himpl_Wp_Triple. applys* M1. }
-  { intros X. rewrite Triple_eq_himpl_Wp_Triple.
+  { rewrite Triple_eq_himpl_Wp. applys* M1. }
+  { intros X. rewrite Triple_eq_himpl_Wp.
     unfold Subst1. rewrite <- isubst_add_eq_subst1_isubst. applys* M2. }
 Qed.
 
-Lemma Wp_sound_app : forall t1 t2,
-  Wp_sound (trm_app t1 t2).
+Lemma Wpgen_sound_app : forall t1 t2,
+  Wpgen_sound (trm_app t1 t2).
 Proof using.
-  intros. intros E A EA. simpl. applys qimpl_Wp_Triple.
+  intros. intros E A EA. simpl. applys qimpl_Wp.
   intros Q. remove_Local. simpl.
-  rewrite Triple_eq_himpl_Wp_Triple. hsimpl.
+  rewrite Triple_eq_himpl_Wp. hsimpl.
 Qed.
 
-Lemma Wp_sound_while : forall F1 F2 E t1 t2,
-  F1 ====> Wp_Triple_ E t1 ->
-  F2 ====> Wp_Triple_ E t2 ->
-  Wp_while F1 F2 ====> Wp_Triple_ E (trm_while t1 t2).
+Lemma Wpgen_sound_while : forall F1 F2 E t1 t2,
+  F1 ====> Wpsubst E t1 ->
+  F2 ====> Wpsubst E t2 ->
+  Wpgen_while F1 F2 ====> Wpsubst E (trm_while t1 t2).
 Proof using.
-  introv M1 M2. intros A EA. applys qimpl_Wp_Triple. intros Q.
+  introv M1 M2. intros A EA. applys qimpl_Wp. intros Q.
   remove_Local. simpl.
   unfold Formula_typed. xpull ;=> Q' C. applys Triple_enc_change (rm C).
-  set (R := Wp_Triple (trm_while (isubst E t1) (isubst E t2))).
+  set (R := Wp (trm_while (isubst E t1) (isubst E t2))).
   applys Triple_hforall R. simpl. applys Triple_hwand_hpure_l.
   { split.
-    { applys @is_local_Wp_Triple. }
-    { clears Q. applys qimpl_Wp_Triple. intros Q.
+    { applys @is_local_Wp. }
+    { clears Q. applys qimpl_Wp. intros Q.
       applys Triple_while_raw.
       asserts_rewrite~ (
          trm_if (isubst E t1) (trm_seq (isubst E t2) (trm_while (isubst E t1) (isubst E t2))) val_unit
        = isubst E (trm_if t1 (trm_seq t2 (trm_while t1 t2)) val_unit)).
-      rewrite Triple_eq_himpl_Wp_Triple. applys~ Wp_sound_if.
-      { applys~ Wp_sound_seq. }
-      { intros A1 EA1 Q''. applys Wp_sound_val. } } }
-  { rewrite~ @Triple_eq_himpl_Wp_Triple. }
+      rewrite Triple_eq_himpl_Wp. applys~ Wpgen_sound_if.
+      { applys~ Wpgen_sound_seq. }
+      { intros A1 EA1 Q''. applys Wpgen_sound_val. } } }
+  { rewrite~ @Triple_eq_himpl_Wp. }
 Qed.
 
-Lemma Wp_sound_for_val : forall (x:var) v1 v2 F1 E t1,
-  (forall X, F1 X ====> Wp_Triple_ (Ctx.add x X E) t1) ->
-  Wp_for_val v1 v2 F1 ====> Wp_Triple_ E (trm_for x v1 v2 t1).
+Lemma Wpgen_sound_for_val : forall (x:var) v1 v2 F1 E t1,
+  (forall X, F1 X ====> Wpsubst (Ctx.add x X E) t1) ->
+  Wpgen_for_val v1 v2 F1 ====> Wpsubst E (trm_for x v1 v2 t1).
 Proof using. Opaque Ctx.add Ctx.rem.
-  introv M. intros A EA. applys qimpl_Wp_Triple. intros Q.
+  introv M. intros A EA. applys qimpl_Wp. intros Q.
   remove_Local. simpl.
   unfold Formula_typed. xpull ;=> Q' n1 n2 (->&->) C.
   applys Triple_enc_change (rm C).
-  set (S := fun (i:int) => Wp_Triple (isubst E (trm_for x i n2 t1))).
+  set (S := fun (i:int) => Wp (isubst E (trm_for x i n2 t1))).
   applys Triple_hforall S. simpl. applys Triple_hwand_hpure_l.
   { split.
-    { intros r. applys @is_local_Wp_Triple. }
-    { clears Q. intros i. applys qimpl_Wp_Triple. intros Q.
+    { intros r. applys @is_local_Wp. }
+    { clears Q. intros i. applys qimpl_Wp. intros Q.
       applys Triple_for_raw. fold isubst.
-      rewrite~ @Triple_eq_himpl_Wp_Triple. case_if.
+      rewrite~ @Triple_eq_himpl_Wp. case_if.
       { unfold Subst1. rewrite <- isubst_add_eq_subst1_isubst.
         asserts_rewrite (trm_seq (isubst (Ctx.add x (``i) E) t1) (trm_for x (i + 1)%I n2 (isubst (Ctx.rem x E) t1))
           = (isubst (Ctx.add x (``i) E) (trm_seq t1 (trm_for x (i + 1)%I n2 t1)))).
         { simpl. rewrite Ctx.rem_anon, Ctx.rem_add_same. auto. }
-        applys Wp_sound_seq.
+        applys Wpgen_sound_seq.
         { applys* M. }
-        { unfold S. unfold Wp_Triple_. simpl. rewrite~ Ctx.rem_add_same. } }
-      { applys Wp_sound_val E. } } }
-  { rewrite~ @Triple_eq_himpl_Wp_Triple. }
+        { unfold S. unfold Wp_. simpl. rewrite~ Ctx.rem_add_same. } }
+      { applys Wpgen_sound_val E. } } }
+  { rewrite~ @Triple_eq_himpl_Wp. }
 Qed.
-
-Lemma himpl_wp_fail_l : forall `{EA:Enc A} (Q:A->hprop) H,
-  ^Wp_fail Q ==> H.
-Proof using. intros. unfold Wp_fail, Local, local. hpull. Qed.
 
 (** Putting it all together *)
 
-Lemma Wp_sound_trm : forall t,
-  Wp_sound t.
+Lemma Wpgen_sound_trm : forall t,
+  Wpgen_sound t.
 Proof using.
   intros t. induction t; intros E A EA Q.
-  { applys Wp_sound_val. }
-  { applys Wp_sound_var. }
-  { applys Wp_sound_fix. }
-  { applys* Wp_sound_if. }
+  { applys Wpgen_sound_val. }
+  { applys Wpgen_sound_var. }
+  { applys Wpgen_sound_fix. }
+  { applys* Wpgen_sound_if. }
   { (* todo factorize? *)
     destruct b as [|x].
-    { applys* Wp_sound_seq. }
-    { applys* Wp_sound_let. } }
-  { applys* Wp_sound_app. }
-  { applys* Wp_sound_while. }
-  { destruct t1; try solve [ applys @himpl_wp_fail_l ].
-    destruct t2; try solve [ applys @himpl_wp_fail_l ].
-    applys* Wp_sound_for_val. }
+    { applys* Wpgen_sound_seq. }
+    { applys* Wpgen_sound_let. } }
+  { applys* Wpgen_sound_app. }
+  { applys* Wpgen_sound_while. }
+  { destruct t1; try solve [ applys @himpl_Wpgen_fail_l ].
+    destruct t2; try solve [ applys @himpl_Wpgen_fail_l ].
+    applys* Wpgen_sound_for_val. }
 Qed.
  *)
-
 
 
 (* ---------------------------------------------------------------------- *)
 (* ** Corrolaries of the soundness of [wp] *)
 
-Lemma Triple_isubst_Wp : forall t E `{EA:Enc A} (Q:A->hprop),
-  Triple (isubst E t) (^(Wp E t) Q) Q.
+Lemma Triple_isubst_Wpgen : forall t E `{EA:Enc A} (Q:A->hprop),
+  Triple (isubst E t) (^(Wpgen E t) Q) Q.
 Proof using. Admitted. (* TODO
-  intros. rewrite Triple_eq_himpl_Wp_Triple. applys Wp_sound_trm.
+  intros. rewrite Triple_eq_himpl_Wp. applys Wpgen_sound_trm.
 Qed.*)
 
-Lemma Triple_isubst_of_Wp : forall t E H `{EA:Enc A} (Q:A->hprop),
-  H ==> ^(Wp E t) Q ->
+Lemma Triple_isubst_of_Wpgen : forall t E H `{EA:Enc A} (Q:A->hprop),
+  H ==> ^(Wpgen E t) Q ->
   Triple (isubst E t) H Q.
-Proof using. introv M. xchanges M. applys Triple_isubst_Wp. Qed.
+Proof using. introv M. xchanges M. applys Triple_isubst_Wpgen. Qed.
 
-Lemma Triple_of_Wp : forall (t:trm) H `{EA:Enc A} (Q:A->hprop),
-  H ==> ^(Wp Ctx.empty t) Q ->
+Lemma Triple_of_Wpgen : forall (t:trm) H `{EA:Enc A} (Q:A->hprop),
+  H ==> ^(Wpgen Ctx.empty t) Q ->
   Triple t H Q.
 Proof using.
   introv M. xchanges M. pattern t at 1; rewrite <- (isubst_empty t).
-  applys Triple_isubst_Wp.
+  applys Triple_isubst_Wpgen.
 Qed.
 
 (* not used *)
-Lemma Wp_Triple_of_Wp : forall t H `{EA:Enc A} (Q:A->hprop),
-  H ==> ^(Wp Ctx.empty t) Q ->
-  H ==> ^(Wp_Triple t) Q.
-Proof using. introv M. applys himpl_weakestpre. applys* Triple_of_Wp. Qed.
+Lemma Wp_of_Wpgen : forall t H `{EA:Enc A} (Q:A->hprop),
+  H ==> ^(Wpgen Ctx.empty t) Q ->
+  H ==> ^(Wp t) Q.
+Proof using. introv M. applys himpl_weakestpre. applys* Triple_of_Wpgen. Qed.
 
-Lemma himpl_wp_app_of_Triple : forall A `{EA:Enc A} (Q:A->hprop) t H,
+(* not used *)
+Lemma himpl_Wpgen_app_of_Triple : forall A `{EA:Enc A} (Q:A->hprop) t H,
   Triple t H Q ->
-  H ==> ^(Wp_app t) Q.
-Proof using. intros. applys Local_erase. rewrite~ <- Triple_eq_himpl_Wp_Triple. Qed.
+  H ==> ^(Wpgen_app t) Q.
+Proof using. intros. applys Local_erase. rewrite~ <- Triple_eq_himpl_Wp. Qed.
 
 
 (* ********************************************************************** *)
@@ -705,11 +584,11 @@ Proof using. intros. applys Local_erase. rewrite~ <- Triple_eq_himpl_Wp_Triple. 
 (* ** Notation for computed WP *)
 
 Notation "'Fail'" :=
-  ((Wp_fail))
+  ((Wpgen_fail))
   (at level 69) : wp_scope.
 
 Notation "'Val' v" :=
-  ((Wp_val v))
+  ((Wpgen_val v))
   (at level 69) : wp_scope.
 
 Notation "'Return' F " :=
@@ -717,95 +596,95 @@ Notation "'Return' F " :=
   (at level 68) : wp_scope.
 
 Notation "'`Let' x ':=' F1 'in' F2" :=
-  ((Wp_let_typed F1 (fun x => F2)))
+  ((Wpgen_let_typed F1 (fun x => F2)))
   (at level 69, x ident, right associativity,
   format "'[v' '[' '`Let'  x  ':='  F1  'in' ']'  '/'  '[' F2 ']' ']'") : wp_scope.
 
 Notation "'Let' [ A EA ] x ':=' F1 'in' F2" :=
-  ((Wp_let F1 (fun A EA x => F2)))
+  ((Wpgen_let F1 (fun A EA x => F2)))
   (at level 69, A at level 0, EA at level 0, x ident, right associativity,
   format "'[v' '[' 'Let'  [ A  EA ]  x  ':='  F1  'in' ']'  '/'  '[' F2 ']' ']'") : wp_scope.
 
 Notation "'Seq' F1 ;;; F2" :=
-  ((Wp_seq F1 F2))
+  ((Wpgen_seq F1 F2))
   (at level 68, right associativity,
    format "'[v' 'Seq'  '[' F1 ']'  ;;;  '/'  '[' F2 ']' ']'") : wp_scope.
 
 Notation "'`Letval' x ':=' v 'in' F2" :=
-  ((Wp_letval_typed v (fun x => F2)))
+  ((Wpgen_letval_typed v (fun x => F2)))
   (at level 69, x ident, right associativity,
   format "'[v' '[' '`Letval'  x  ':='  v  'in' ']'  '/'  '[' F2 ']' ']'") : wp_scope.
 
 Notation "'Letval' [ A EA ] x ':=' v 'in' F2" :=
-  ((Wp_letval v (fun A EA x => F2)))
+  ((Wpgen_letval v (fun A EA x => F2)))
   (at level 69, A at level 0, EA at level 0, x ident, right associativity,
   format "'[v' '[' 'Letval'  [ A  EA ]  x  ':='  v  'in' ']'  '/'  '[' F2 ']' ']'") : wp_scope.
  
 (*
 Notation "'App' f t1 " :=
-  (Wp_app (trm_apps f (t1::nil)))
+  (Wpgen_app (trm_apps f (t1::nil)))
   (at level 68, f, t1 at level 0) : wp_scope.
 
 Notation "'App' f t1 t2 " :=
-  (Wp_app (trm_apps f (t1::t2::nil)))
+  (Wpgen_app (trm_apps f (t1::t2::nil)))
   (at level 68, f, t1, t2 at level 0) : wp_scope.
 
 Notation "'App' f t1 t2 t3 " :=
-  (Wp_app (trm_apps f (t1::t2::t3::nil)))
+  (Wpgen_app (trm_apps f (t1::t2::t3::nil)))
   (at level 68, f, t1, t2, t3 at level 0) : wp_scope.
 *)
 
 Notation "'App' f v1 " :=
-  ((Wp_app (trm_apps f (trms_vals (v1::nil)))))
+  ((Wpgen_app (trm_apps f (trms_vals (v1::nil)))))
   (at level 68, f, v1 at level 0) : wp_scope.
 
 Notation "'App' f v1 v2 " :=
-  ((Wp_app (trm_apps f (trms_vals (v1::v2::nil)))))
+  ((Wpgen_app (trm_apps f (trms_vals (v1::v2::nil)))))
   (at level 68, f, v1, v2 at level 0) : wp_scope.
 
 Notation "'App' f v1 v2 v3 " :=
-  ((Wp_app (trm_apps f (trms_vals (v1::v2::v3::nil)))))
+  ((Wpgen_app (trm_apps f (trms_vals (v1::v2::v3::nil)))))
   (at level 68, f, v1, v2, v3 at level 0) : wp_scope.
 
 (* TODO: recursive notation for App *)
 
 Notation "'Ifval' b 'Then' F1 'Else' F2" :=
-  ((Wp_if_val b F1 F2))
+  ((Wpgen_if_val b F1 F2))
   (at level 69) : wp_scope.
 
 (* DEPRECATED
 Notation "'If' F0 'Then' F1 'Else' F2" :=
-  ((Wp_if F0 F1 F2))
+  ((Wpgen_if F0 F1 F2))
   (at level 69, F0 at level 0) : wp_scope.
 *)
 
 Notation "'While' F1 'Do' F2 'Done'" :=
-  ((Wp_while F1 F2))
+  ((Wpgen_while F1 F2))
   (at level 69, F2 at level 68,
    format "'[v' 'While'  F1  'Do'  '/' '[' F2 ']' '/'  'Done' ']'")
    : wp_scope.
 
 Notation "'For' x '=' n1 'To' n2 'Do' F3 'Done'" :=
-  ((Wp_for_int n1 n2 (fun x => F3)))
+  ((Wpgen_for_int n1 n2 (fun x => F3)))
   (at level 69, x ident,
    format "'[v' 'For'  x  '='  n1  'To'  n2  'Do'  '/' '[' F3 ']' '/'  'Done' ']'")
   : wp_scope.
 
 
 Notation "'Case' v '=' vp ''=>' F1 ''|' F2" :=
-  ((Wp_case_val (fun A EA Q => \[v = vp%val] \-* F1 A EA Q) (v <> vp%val) F2))
+  ((Wpgen_case_val (fun A EA Q => \[v = vp%val] \-* F1 A EA Q) (v <> vp%val) F2))
   (at level 69, v, vp at level 69,
    format "'[v' 'Case'  v  '='  vp  ''=>'  '[' '/' F1 ']' '[' '/'  ''|'  F2 ']' ']'")
    : wp_scope.
 
 Notation "'Case' v '=' vp [ x1 ] ''=>' F1 ''|' F2" :=
-  ((Wp_case_val (fun A EA Q => \forall x1, \[v = vp%val] \-* F1 A EA Q) (forall x1, v <> vp%val) F2))
+  ((Wpgen_case_val (fun A EA Q => \forall x1, \[v = vp%val] \-* F1 A EA Q) (forall x1, v <> vp%val) F2))
   (at level 69, v, vp at level 69, x1 ident,
    format "'[v' 'Case'  v  '='  vp  [ x1 ]  ''=>'  '[' '/' F1 ']' '[' '/'  ''|'  F2 ']' ']'")
    : wp_scope.
 
 Notation "'Case' v '=' vp [ x1 x2 ] ''=>' F1 ''|' F2" :=
-  ((Wp_case_val (fun A EA Q => \forall x1 x2, \[v = vp%val] \-* F1 A EA Q) (forall x1 x2, v <> vp%val) F2))
+  ((Wpgen_case_val (fun A EA Q => \forall x1 x2, \[v = vp%val] \-* F1 A EA Q) (forall x1 x2, v <> vp%val) F2))
   (at level 69, v, vp at level 69, x1 ident, x2 ident,
    format "'[v' 'Case'  v  '='  vp  [ x1  x2 ]  ''=>'  '[' '/' F1 ']' '[' '/'  ''|'  F2 ']' ']'")
    : wp_scope.
@@ -814,27 +693,27 @@ Notation "'Case' v '=' vp [ x1 x2 ] ''=>' F1 ''|' F2" :=
 (* DEPRECATED
 Notation "'Match_' v 'With' ''|' vp1 ''=>' F1 ''|' vp2 ''=>' F2" :=
   (Case v = vp1%val Then F1 Else 
-   is_Wp (Case v = vp2%val Then F2 Else 
-   is_Wp (Fail))) (at level 69, v, vp1, vp2 at level 69,
+   Wptag (Case v = vp2%val Then F2 Else 
+   Wptag (Fail))) (at level 69, v, vp1, vp2 at level 69,
    format "'[v' 'Match_'  v  'With'  '[' '/' ''|'  vp1  ''=>'  '/' F1 ']'  '[' '/' ''|'  vp2  ''=>'  '/' F2 ']' ']'")
   : wp_scope.
 
 Notation "'Match_' v 'With' ''|' vp1 ''=>' F1 ''|' vp2 [ x21 ] ''=>' F2" :=
   (Case v = vp1%val Then F1 Else 
-   is_Wp (Case v = vp2%val [ x21 ] Then F2 Else 
-   is_Wp (Fail))) (at level 69, v, vp1, vp2 at level 69, x21 ident,
+   Wptag (Case v = vp2%val [ x21 ] Then F2 Else 
+   Wptag (Fail))) (at level 69, v, vp1, vp2 at level 69, x21 ident,
    format "'[v' 'Match_'  v  'With'  '[' '/' ''|'  vp1  ''=>'  '/' F1 ']'  '[' '/' ''|'  vp2  [ x21 ]  ''=>'  '/' F2 ']' ']'")
   : wp_scope.
 
 Notation "'Match_' v 'With' ''|' vp1 ''=>' F1 ''|' vp2 [ x21 x22 ] ''=>' F2" :=
   (Case v = vp1%val Then F1 Else 
-   is_Wp (Case v = vp2%val [ x21 x22 ] Then F2 Else 
-   is_Wp (Fail))) (at level 69, v, vp1, vp2 at level 0, x21 ident, x22 ident,
+   Wptag (Case v = vp2%val [ x21 x22 ] Then F2 Else 
+   Wptag (Fail))) (at level 69, v, vp1, vp2 at level 0, x21 ident, x22 ident,
    format "'[v' 'Match_'  v  'With'  '[' '/' ''|'  vp1  ''=>'  '/' F1 ']'  '[' '/' ''|'  vp2  [ x21  x22 ]  ''=>'  '/' F2 ']' ']'")
   : wp_scope.
 
 Notation "'Match_' v 'With' Fof 'End'" :=
-  ((Wp_match_val v Fof))
+  ((Wpgen_match_val v Fof))
   (at level 69,
    format "'[v' 'Match_'  v  'With'  '/' '[' Fof ']' '/'  'End' ']'")
    : wp_scope.
@@ -845,7 +724,7 @@ Notation "'Match_' v 'With' Fof 'End'" :=
 
 (* NEEDED?
 Notation "'Apptrm' t " :=
-  ((Wp_app t))
+  ((Wpgen_app t))
   (at level 68, t at level 0) : wp_scope.
 *)
 
