theories/WPRecord.v
@@ -348,19 +348,19 @@ Ltac xspec_record tt :=
 Lemma xapp_record_get : forall A `{EA:Enc A} (Q:A->hprop) (H:hprop) (p:loc) (f:field) (L:Record_fields),
   H ==> p ~> Record L \* (match record_get_compute_dyn f L with
     | None => \[False]
-    | Some (Dyn V) => (p ~> Record L) \-* ^(is_Wp (Wp_cast V)) (protect Q) end) ->
-  H ==> ^(Wp_app (trm_apps (trm_val (val_get_field f)) (trms_vals ((p:val)::nil)))) Q.
+    | Some (Dyn V) => (p ~> Record L) \-* ^(Wptag (Wpgen_cast V)) (protect Q) end) ->
+  H ==> ^(Wpgen_app (trm_apps (trm_val (val_get_field f)) (trms_vals ((p:val)::nil)))) Q.
 Proof using.
   introv M1. hchanges (rm M1).
   lets R: record_get_compute_spec_correct f L.
   unfolds record_get_compute_spec.
   destruct (record_get_compute_dyn f L) as [[T ET V]|]; try solve [hpull].  
-  set (H' := (p ~> Record L \-* ^(`Wp_cast V) Q)).
+  set (H' := (p ~> Record L \-* ^(`Wpgen_cast V) Q)).
   forwards R': R; eauto. clear R. specializes R' p.
-  applys himpl_wp_app_of_Triple.
+  applys himpl_Wpgen_app_of_Triple.
   applys Triple_enc_change. xapplys (rm R'). simpl.
-  unfold PostChange, is_Wp. hpull ;=> ? ->. unfold H'. hpull.
-  unfold Wp_cast, is_Wp. applys himpl_refl.
+  unfold RetypePost, Wptag. hpull ;=> ? ->. unfold H'. hpull.
+  unfold Wpgen_cast, Wptag. applys himpl_refl.
 Qed. (* TODO: simplify proof *)
 
 Lemma xapp_record_set : forall A1 `{EA1:Enc A1} (W:A1) (Q:unit->hprop) (H:hprop) (p:loc) (f:field) (L:Record_fields),
@@ -369,14 +369,14 @@ Lemma xapp_record_set : forall A1 `{EA1:Enc A1} (W:A1) (Q:unit->hprop) (H:hprop)
     | None => \[False]
     | Some L' =>  
         (p ~> Record L' \-* protect (Q tt)) end)  ) ->
-  H ==> ^(Wp_app (trm_apps (trm_val (val_set_field f)) (trms_vals ((p:val)::(``W)::nil)))) Q.
+  H ==> ^(Wpgen_app (trm_apps (trm_val (val_set_field f)) (trms_vals ((p:val)::(``W)::nil)))) Q.
 Proof using.
   introv M1. hchanges (rm M1).
   lets R: record_set_compute_spec_correct f W L.
   unfolds record_set_compute_spec.
   destruct (record_set_compute_dyn f (Dyn W) L) as [L'|]; try solve [hpull].
   forwards R': R; eauto. clear R. specializes R' p. 
-  applys himpl_wp_app_of_Triple.
+  applys himpl_Wpgen_app_of_Triple.
   xapplys R'.
 Qed. (* TODO: simplify proof *)
 
