theories/WPTactics.v
@@ -35,12 +35,12 @@ Implicit Types H : hprop.
 (** Display [H ==> ^F Q] as [PRE H CODE F POST Q] *)
 
 (* DEPRECATED
-Notation "'CODE' F 'POST' Q" := ((is_Wp F) _ _ Q)
+Notation "'CODE' F 'POST' Q" := ((Wptag F) _ _ Q)
   (at level 8, F, Q at level 0,
    format "'[v' 'CODE'  F '/' 'POST'  Q ']'") : wp_scope.
    *)
 
-Notation "'PRE' H 'CODE' F 'POST' Q" := (H ==> (is_Wp F) _ _ Q)
+Notation "'PRE' H 'CODE' F 'POST' Q" := (H ==> (Wptag F) _ _ Q)
   (at level 8, H, F, Q at level 0,
    format "'[v' 'PRE'  H  '/' 'CODE'  F '/' 'POST'  Q ']'") : wp_scope.
 
@@ -80,19 +80,19 @@ Open Scope triple_scope.
 Ltac xgoal_code tt :=
   match goal with |- PRE _ CODE ?C POST _ => constr:(C) end.
 
-Ltac xgoal_code_strip_iswp C :=
+Ltac xgoal_code_strip_wptag C :=
   match C with
-  | is_Wp ?C' => xgoal_code_strip_iswp C'
+  | Wptag ?C' => xgoal_code_strip_wptag C'
   | ?C' => constr:(C')
   end.
 
-Ltac xgoal_code_without_iswp tt :=
+Ltac xgoal_code_without_wptag tt :=
   let C := xgoal_code tt in
-  xgoal_code_strip_iswp C.
+  xgoal_code_strip_wptag C.
 
 Ltac xgoal_fun tt :=
-  match xgoal_code_without_iswp tt with 
-  | Wp_app (trm_apps (trm_val ?f) _) => constr:(f)
+  match xgoal_code_without_wptag tt with 
+  | Wpgen_app (trm_apps (trm_val ?f) _) => constr:(f)
   end.
 
 
@@ -193,8 +193,8 @@ Ltac xwp_simpl :=
   cbn beta delta [ 
   LibList.combine 
   List.rev Datatypes.app List.fold_right List.map
-  Wp WP_getval WP_getval_typed WP_getval_val WP_getval_int
-  WP_apps WP_apps_or_prim WP_constr WP_var WP_match  
+  Wpgen Wpaux_getval Wpaux_getval_typed Wpaux_getval_val Wpaux_getval_int
+  Wpaux_apps Wpaux_apps_or_prim Wpaux_constr Wpaux_var Wpaux_match  
   hforall_vars forall_vars
   trm_case trm_to_pat patvars patsubst combiner_to_trm
   Ctx.app Ctx.empty Ctx.lookup Ctx.add 
@@ -212,26 +212,26 @@ Lemma xwp_lemma_funs : forall F vs ts xs t `{EA:Enc A} H (Q:A->hprop),
   F = val_funs xs t ->
   trms_to_vals ts = Some vs ->
   var_funs_exec (length vs) xs ->
-  H ==> ^(Wp (combine xs vs) t) Q ->
+  H ==> ^(Wpgen (combine xs vs) t) Q ->
   Triple (trm_apps F ts) H Q.
 Proof using.
   introv HF Hvs Hxs M. lets ->: trms_to_vals_spec Hvs.
   rewrite var_funs_exec_eq in Hxs. rew_istrue in Hxs. lets (_&Lxs&_): Hxs.
   applys* Triple_apps_funs. rewrite~ <- isubstn_eq_substn.
-  applys* Triple_isubst_of_Wp.
+  applys* Triple_isubst_of_Wpgen.
 Qed.
 
 Lemma xwp_lemma_fixs : forall F (f:var) vs ts xs t `{EA:Enc A} H (Q:A->hprop),
   F = val_fixs f xs t ->
   trms_to_vals ts = Some vs ->
   var_fixs_exec f (length vs) xs ->
-  H ==> ^(Wp (combine (f::xs) (F::vs)) t) Q ->
+  H ==> ^(Wpgen (combine (f::xs) (F::vs)) t) Q ->
   Triple (trm_apps F ts) H Q.
 Proof using.
   introv HF Hvs Hxs M. lets ->: trms_to_vals_spec Hvs.
   rewrite var_fixs_exec_eq in Hxs. rew_istrue in Hxs. lets (_&Lxs&_): Hxs.
   applys* Triple_apps_fixs. rewrite <- isubstn_eq_substn; [|rew_list~].
-  applys* Triple_isubst_of_Wp.
+  applys* Triple_isubst_of_Wpgen.
 Qed.
 
 Ltac xwp_fun tt :=
@@ -254,8 +254,8 @@ Tactic Notation "xwp" :=
 (* ** Tactic [xseq] *)
 
 Ltac xseq_pre tt :=
-  match xgoal_code_without_iswp tt with
-  | (Wp_seq _ _) => idtac 
+  match xgoal_code_without_wptag tt with
+  | (Wpgen_seq _ _) => idtac 
   end.
 
 Definition xseq_lemma := @Local_erase.
@@ -273,7 +273,7 @@ Tactic Notation "xseq" :=
 
 Lemma xlet_lemma : forall A1 (EA1:Enc A1) H `{EA:Enc A} (Q:A->hprop) (F1:Formula) (F2of:forall `{EA1:Enc A2},A2->Formula),
   H ==> ^F1 (fun (X:A1) => ^(F2of X) Q) -> 
-  H ==> ^(Wp_let F1 (@F2of)) Q.
+  H ==> ^(Wpgen_let F1 (@F2of)) Q.
 Proof using. introv M. applys Local_erase. hsimpl* A1 EA1. Qed.
 
 Definition xlet_typed_lemma := @Local_erase.
@@ -285,9 +285,9 @@ Ltac xlet_typed tt :=
   applys xlet_typed_lemma.
 
 Ltac xlet_core tt :=
-  match xgoal_code_without_iswp tt with
-  | (Wp_let_typed _ _) => xlet_typed tt
-  | (Wp_let _ _) => xlet_poly tt
+  match xgoal_code_without_wptag tt with
+  | (Wpgen_let_typed _ _) => xlet_typed tt
+  | (Wpgen_let _ _) => xlet_poly tt
   end.
 
 Tactic Notation "xlet" :=
@@ -298,14 +298,14 @@ Tactic Notation "xlet" :=
 (* ** Tactic [xcast] *)
 
 Ltac xcast_pre tt :=
-  match xgoal_code_without_iswp tt with
-  | (Wp_cast _) => idtac 
+  match xgoal_code_without_wptag tt with
+  | (Wpgen_cast _) => idtac 
   end.
 
 Lemma xcast_lemma : forall (H:hprop) `{Enc A} (Q:A->hprop) (X:A),
   H ==> Q X ->
-  H ==> ^(Wp_cast X) Q.
-Proof using. introv M. unfold is_Wp, Wp_cast. hchanges~ M. Qed.
+  H ==> ^(Wpgen_cast X) Q.
+Proof using. introv M. unfold Wptag, Wpgen_cast. hchanges~ M. Qed.
 
 Ltac xcast_core tt :=
   xcast_pre tt;
@@ -319,11 +319,11 @@ Tactic Notation "xcast" :=
 (* ** Tactic [xlet_xseq_xcast_repeat] *)
 
 Ltac xlet_xseq_xcast tt :=
-  match xgoal_code_without_iswp tt with
-  | (Wp_let_typed _ _) => xlet
-  | (Wp_let _ _) => xlet
-  | (Wp_seq _ _) => xseq
-  | (Wp_cast _) => xseq
+  match xgoal_code_without_wptag tt with
+  | (Wpgen_let_typed _ _) => xlet
+  | (Wpgen_let _ _) => xlet
+  | (Wpgen_seq _ _) => xseq
+  | (Wpgen_cast _) => xseq
   end.
 
 Ltac xlet_xseq_xcast_repeat tt :=
@@ -360,18 +360,18 @@ Ltac xapp_record tt :=
 Lemma xapp_lemma : forall A `{EA:Enc A} (Q1:A->hprop) t H1 H Q,
   Triple t H1 Q1 ->
   H ==> H1 \* (Q1 \--* protect Q) ->
-  H ==> ^(Wp_app t) Q.
+  H ==> ^(Wpgen_app t) Q.
 Proof using.
   introv M1 M2. applys Local_erase.
   hchanges (rm M2).
-  rewrite <- Triple_eq_himpl_Wp_Triple.
+  rewrite <- Triple_eq_himpl_Wp.
   applys* Triple_ramified_frame.
 Qed.
 
 Lemma xapps_lemma : forall A `{EA:Enc A} (V:A) H2 t H1 H Q,
   Triple t H1 (fun r => \[r = V] \* H2) ->
   H ==> H1 \* (H2 \-* protect (Q V)) ->
-  H ==> ^(Wp_app t) Q.
+  H ==> ^(Wpgen_app t) Q.
 Proof using.
   introv M1 M2. applys xapp_lemma M1. hchanges M2.
   intros ? ->. auto.
@@ -380,19 +380,19 @@ Qed.
 Lemma xapps_lemma_pure : forall A `{EA:Enc A} (V:A) t H1 H Q,
   Triple t H1 (fun r => \[r = V]) ->
   H ==> H1 \* protect (Q V) ->
-  H ==> ^(Wp_app t) Q.
+  H ==> ^(Wpgen_app t) Q.
 Proof using.
   introv M1 M2. applys xapps_lemma \[]; rew_heap; eauto.
 Qed.
 
 (* [xapp_pre tt] automatically performs the necessary 
    [xlet], [xseq] and [xcast], then checks that the goal 
-   is a [Wp_app] goal. *)
+   is a [Wpgen_app] goal. *)
 
 Ltac xapp_pre tt :=
   xlet_xseq_xcast_repeat tt; 
-  match xgoal_code_without_iswp tt with
-  | (Wp_app _) => idtac 
+  match xgoal_code_without_wptag tt with
+  | (Wpgen_app _) => idtac 
   end.
 
 Ltac xapp_post tt :=
@@ -400,8 +400,8 @@ Ltac xapp_post tt :=
   
 Lemma xapp_find_spec_lemma : forall A `{EA:Enc A} (Q1:A->hprop) t H1 H Q,
   Triple t H1 Q1 ->
-  (Triple t H1 Q1 -> H ==> ^(Wp_app t) Q) ->
-  H ==> ^(Wp_app t) Q.
+  (Triple t H1 Q1 -> H ==> ^(Wpgen_app t) Q) ->
+  H ==> ^(Wpgen_app t) Q.
 Proof using. auto. Qed.
 
 Ltac xapp_select_lemma tt :=
@@ -507,24 +507,24 @@ Tactic Notation "xappn" "*" constr(n) :=
 Lemma xval_lemma : forall `{EA:Enc A} (V:A) v H (Q:A->hprop),
   v = ``V ->
   H ==> Q V ->
-  H ==> ^(Wp_val v) Q.
+  H ==> ^(Wpgen_val v) Q.
 Proof using. introv E N. subst. applys Local_erase. hsimpl~ V. Qed.
 
 (* NEEDED? *)
 Lemma xval_lemma_val : forall `{EA:Enc A} (V:A) v H (Q:val->hprop),
   v = ``V ->
   H ==> Q (``V) ->
-  H ==> ^(Wp_val v) Q.
+  H ==> ^(Wpgen_val v) Q.
 Proof using. introv E N. subst. applys Local_erase. hsimpl~ (``V). Qed.
 
 (* [xval_pre tt] automatically performs the necessary 
    [xlet], [xseq] and [xcast], then checks that the goal 
-   is a [Wp_val] goal. *)
+   is a [Wpgen_val] goal. *)
 
 Ltac xval_pre tt :=
   xlet_xseq_xcast_repeat tt; 
-  match xgoal_code_without_iswp tt with
-  | (Wp_val _) => idtac 
+  match xgoal_code_without_wptag tt with
+  | (Wpgen_val _) => idtac 
   end.
 
 Ltac xval_arg E :=
@@ -555,20 +555,20 @@ Tactic Notation "xval" "*"  :=
 
 Ltac xif_pre tt :=
   xlet_xseq_xcast_repeat tt; 
-  match xgoal_code_without_iswp tt with
-  | (Wp_if_val _ _ _) => idtac 
+  match xgoal_code_without_wptag tt with
+  | (Wpgen_if_val _ _ _) => idtac 
   end.
 
 Lemma xifval_lemma : forall `{EA:Enc A} b H (Q:A->hprop) (F1 F2:Formula),
   (b = true -> H ==> ^F1 Q) ->
   (b = false -> H ==> ^F2 Q) ->
-  H ==> ^(Wp_if_val b F1 F2) Q.
+  H ==> ^(Wpgen_if_val b F1 F2) Q.
 Proof using. introv E N. applys Local_erase. case_if*. Qed.
 
 Lemma xifval_lemma_isTrue : forall `{EA:Enc A} (P:Prop) H (Q:A->hprop) (F1 F2:Formula),
   (P -> H ==> ^F1 Q) ->
   (~ P -> H ==> ^F2 Q) ->
-  H ==> ^(Wp_if_val (isTrue P) F1 F2) Q.
+  H ==> ^(Wpgen_if_val (isTrue P) F1 F2) Q.
 Proof using. introv E N. applys Local_erase. case_if*. Qed.
 
 Ltac xif_core tt :=
@@ -584,14 +584,14 @@ Tactic Notation "xif" :=
 
 Ltac xcase_pre tt :=
   xlet_xseq_xcast_repeat tt; 
-  match xgoal_code_without_iswp tt with
-  | (Wp_case_val _ _ _) => idtac 
+  match xgoal_code_without_wptag tt with
+  | (Wpgen_case_val _ _ _) => idtac 
   end.
 
 Lemma xcase_lemma : forall F1 (P:Prop) F2 H `{EA:Enc A} (Q:A->hprop),
   (H ==> ^F1 Q) ->
   (P -> H ==> ^F2 Q) ->
-  H ==> ^(Wp_case_val F1 P F2) Q.
+  H ==> ^(Wpgen_case_val F1 P F2) Q.
 Proof using. 
   introv M1 M2. apply Local_erase. applys himpl_hand_r. 
   { auto. }
@@ -601,7 +601,7 @@ Qed.
 Lemma xcase_lemma0 : forall F1 (P1 P2:Prop) F2 H `{EA:Enc A} (Q:A->hprop),
   (P1 -> H ==> ^F1 Q) ->
   (P2 -> H ==> ^F2 Q) ->
-  H ==> ^(Wp_case_val (fun `{EA1:Enc A1} (Q:A1->hprop) => \[P1] \-* ^F1 Q) P2 F2) Q.
+  H ==> ^(Wpgen_case_val (fun `{EA1:Enc A1} (Q:A1->hprop) => \[P1] \-* ^F1 Q) P2 F2) Q.
 Proof using. 
   introv M1 M2. applys* xcase_lemma. { applys* hwand_move_l_pure. }
 Qed.
@@ -609,7 +609,7 @@ Qed.
 Lemma xcase_lemma2 : forall (F1:val->val->Formula) (P1:val->val->Prop) (P2:Prop) F2 H `{EA:Enc A} (Q:A->hprop),
   (forall x1 x2, P1 x1 x2 -> H ==> ^(F1 x1 x2) Q) ->
   (P2 -> H ==> ^F2 Q) ->
-  H ==> ^(Wp_case_val (fun `{EA1:Enc A1} (Q:A1->hprop) => \forall x1 x2, \[P1 x1 x2] \-* ^(F1 x1 x2) Q) P2 F2) Q.
+  H ==> ^(Wpgen_case_val (fun `{EA1:Enc A1} (Q:A1->hprop) => \forall x1 x2, \[P1 x1 x2] \-* ^(F1 x1 x2) Q) P2 F2) Q.
 Proof using. 
   introv M1 M2. applys* xcase_lemma.
   { repeat (applys himpl_hforall_r ;=> ?). applys* hwand_move_l_pure. }
@@ -654,7 +654,7 @@ Lemma xreturn_lemma_typed : forall `{Enc A1} (F:(A1->hprop)->hprop) (Q:A1->hprop
   H ==> F Q ->
   H ==> ^(Formula_typed F) Q.
 Proof using.
-  introv M. unfold Formula_typed. hsimpl* Q. applys PostChange_refl.
+  introv M. unfold Formula_typed. hsimpl* Q. applys RetypePost_refl.
 Qed.
 
 Lemma xreturn_lemma_val : forall `{Enc A1} (F:(A1->hprop)->hprop) (Q:val->hprop) H,
@@ -662,7 +662,7 @@ Lemma xreturn_lemma_val : forall `{Enc A1} (F:(A1->hprop)->hprop) (Q:val->hprop)
   H ==> ^(Formula_typed F) Q.
 Proof using.
   introv M. unfold Formula_typed. hsimpl* Q.
-  unfold PostChange. intros X. hsimpl* X.
+  unfold RetypePost. intros X. hsimpl* X.
 Qed.
 
 
